Velvet2/Basic.lean
@@ -3,3 +3,4 @@ import Velvet2.Syntax
 import Velvet2.Tactics
 import Velvet2.Examples.Examples
 import Velvet2.Examples.FibExperiment
+import Velvet2.Examples.StateT
